IMP-_To_SAS+/IMP_Minus_To_SAS_Plus.thy
@@ -23,13 +23,47 @@ definition max_input_bits:: "IMP_Minus_com \<Rightarrow> (vname \<rightharpoonup
 "max_input_bits c I r = 
   bit_length (max (max (Max (ran I)) r) (IMP_Minus_Max_Constant.max_constant c))" 
 
+lemma bit_at_index_geq_max_input_bits_is_zero: "x < r \<Longrightarrow> max_input_bits c I r \<le> b  
+  \<Longrightarrow> nth_bit x b = Zero" 
+  sorry
+
+lemma bit_at_index_geq_max_input_bits_is_zero_in_initial_state: "finite (ran I) 
+  \<Longrightarrow> max_input_bits c I r \<le> b
+  \<Longrightarrow> I x = Some y \<Longrightarrow> nth_bit y b = Zero"
+  sorry
+
+lemma max_constant_less_two_to_the_max_input_bits: "max_constant c < 2 ^ (max_input_bits c I r)" 
+  apply(auto simp: max_input_bits_def bit_length_def algebra_simps)
+  using log_exp2_gt max_less_iff_conj by blast
+
+lemma initial_state_element_less_two_to_the_max_input_bits: 
+  assumes "finite (ran I)" "I x = Some y" 
+  shows "y < (2 :: nat) ^ (max_input_bits c I r)" 
+proof -
+  have "y \<le> Max (ran I)" using assms by (meson Max_ge ranI)
+  thus ?thesis using log_exp2_gt max_less_iff_conj
+    by(fastforce simp: max_input_bits_def bit_length_def algebra_simps)
+qed
+
+definition IMP_Minus_initial_to_IMP_Minus_Minus:: "(vname \<rightharpoonup> nat) 
+  \<Rightarrow> nat \<Rightarrow> nat \<Rightarrow> (vname \<rightharpoonup> bit)" where
+"IMP_Minus_initial_to_IMP_Minus_Minus I n guess_range = (\<lambda>v. 
+  (case var_to_operand_bit v of 
+    Some (CHR ''a'', k) \<Rightarrow> if k < n then Some Zero else None |
+    Some (CHR ''b'', k) \<Rightarrow> if k < n then Some Zero else None | 
+    _ \<Rightarrow> (if v = ''carry'' then Some Zero 
+  else (IMP_Minus_State_To_IMP_Minus_Minus_partial I n guess_range) v)))" 
+
+
 definition IMP_Minus_to_SAS_Plus:: "IMP_Minus_com \<Rightarrow> (vname \<rightharpoonup> nat) \<Rightarrow> nat \<Rightarrow> (vname \<rightharpoonup> nat) 
   \<Rightarrow>  nat \<Rightarrow> SAS_problem" where
 "IMP_Minus_to_SAS_Plus c I r G t = (let 
-  n = t + max_input_bits c I r + 1;
+  guess_range = max_input_bits c I r;
+  n = t + guess_range + 1;
   c' = IMP_Minus_To_IMP_Minus_Minus c n;
-  I' = (IMP_Minus_State_To_IMP_Minus_Minus_partial I n) |` (set (enumerate_variables c')) ;
-  G' = (IMP_Minus_State_To_IMP_Minus_Minus_partial G n) |` (set (enumerate_variables c')) in 
+  I' = IMP_Minus_initial_to_IMP_Minus_Minus I n guess_range
+    |` (set (enumerate_variables c')) ;
+  G' = (IMP_Minus_State_To_IMP_Minus_Minus_partial G n n) |` (set (enumerate_variables c')) in 
   SAS_Plus_Plus_To_SAS_Plus (imp_minus_minus_to_sas_plus c' I' G'))"
 
 lemma le_mul_intro: "0 < b \<Longrightarrow> a \<le> b \<Longrightarrow> (1 :: nat) < c \<Longrightarrow> a < c * b" 
@@ -46,12 +80,15 @@ lemma IMP_Minus_to_SAS_Plus_correctness:
       + (max_input_bits c I r + t + 1 + 1) * (num_variables c + 2) + 52
       \<and> is_serial_solution_for_problem (IMP_Minus_to_SAS_Plus c I r G t) plan"
 proof -
-  let ?n = "t + max_input_bits c I r + 1"
+  let ?guess_range = " max_input_bits c I r"
+  let ?n = "t + ?guess_range + 1"
   let ?c' = "IMP_Minus_To_IMP_Minus_Minus c ?n"
   let ?s1' = "IMP_Minus_State_To_IMP_Minus_Minus s1 ?n |` (set (enumerate_variables ?c'))"
   let ?s2' = "IMP_Minus_State_To_IMP_Minus_Minus s2 ?n |` (set (enumerate_variables ?c'))"
-  let ?I = "(IMP_Minus_State_To_IMP_Minus_Minus_partial I ?n) |` (set (enumerate_variables ?c'))"
-  let ?G = "(IMP_Minus_State_To_IMP_Minus_Minus_partial G ?n) |` (set (enumerate_variables ?c'))"
+  let ?I = "(IMP_Minus_initial_to_IMP_Minus_Minus I ?n ?guess_range) 
+    |` (set (enumerate_variables ?c'))"
+  let ?G = "(IMP_Minus_State_To_IMP_Minus_Minus_partial G ?n ?n) 
+    |` (set (enumerate_variables ?c'))"
   let ?t = "100 * ?n * (t - 1) + 51"
   let ?sas_plus_plus_problem 
     = "imp_minus_minus_to_sas_plus (IMP_Minus_To_IMP_Minus_Minus c ?n) ?I ?G"
@@ -72,11 +109,27 @@ proof -
 
   hence "?G v = Some y \<Longrightarrow> ?s2' v = Some y" for v y
     using \<open>G \<subseteq>\<^sub>m Some \<circ> s2\<close> 
-      by(auto simp: IMP_Minus_State_To_IMP_Minus_Minus_def  
+    apply(auto simp: IMP_Minus_State_To_IMP_Minus_Minus_def var_to_var_bit_eq_Some_iff
           IMP_Minus_State_To_IMP_Minus_Minus_with_operands_a_b_def 
            IMP_Minus_State_To_IMP_Minus_Minus_partial_def map_le_def map_comp_def dom_def
            split!: option.splits if_splits char.splits bool.splits)
+    apply(frule var_bit_in_IMP_Minus_Minus_variables_then_bit_less_n)
+    by simp
   hence "?G \<subseteq>\<^sub>m ?s2'" by (auto simp: map_le_def)
+
+  have "?I v = Some y \<Longrightarrow> ?s1' v = Some y" for v y
+    apply auto
+    apply(drule set_mp[OF IMP_Minus_To_IMP_Minus_Minus_variables])
+    apply(cases "v = ''carry''")
+    using \<open>I \<subseteq>\<^sub>m Some \<circ> s1\<close>
+     apply(auto simp: IMP_Minus_State_To_IMP_Minus_Minus_partial_def 
+        IMP_Minus_State_To_IMP_Minus_Minus_with_operands_a_b_def dom_def
+        IMP_Minus_State_To_IMP_Minus_Minus_def map_comp_def map_le_def 
+        IMP_Minus_initial_to_IMP_Minus_Minus_def
+        split: if_splits option.splits)
+    using \<open>finite (range s1)\<close> \<open>Max (range s1) < r\<close> 
+    by(auto intro: bit_at_index_geq_max_input_bits_is_zero)
+  hence "?I  \<subseteq>\<^sub>m ?s1'" by (auto simp: map_le_def)
 
   let ?ss1'' = "imp_minus_state_to_sas_plus (?c', ?s1')" 
   let ?ss2'' = "imp_minus_state_to_sas_plus (SKIP, ?s2')" 
@@ -87,13 +140,8 @@ proof -
             where ?I="?I" and ?G="?G"]])
        apply auto
       apply(drule set_mp[OF IMP_Minus_To_IMP_Minus_Minus_variables])
-      apply(auto simp: IMP_Minus_State_To_IMP_Minus_Minus_def 
-        IMP_Minus_State_To_IMP_Minus_Minus_with_operands_a_b_def)[1]
-     apply(auto simp: map_le_def)[1]
-     apply(drule set_mp[OF IMP_Minus_To_IMP_Minus_Minus_variables])
-    using \<open>I \<subseteq>\<^sub>m Some \<circ> s1\<close> \<open>?G \<subseteq>\<^sub>m ?s2'\<close> by(auto simp:  IMP_Minus_State_To_IMP_Minus_Minus_def 
-        IMP_Minus_State_To_IMP_Minus_Minus_partial_def map_comp_Some_iff map_le_def dom_def
-        IMP_Minus_State_To_IMP_Minus_Minus_with_operands_a_b_def)+
+      using \<open>?I  \<subseteq>\<^sub>m ?s1'\<close> \<open>?G \<subseteq>\<^sub>m ?s2'\<close> by(auto simp: IMP_Minus_State_To_IMP_Minus_Minus_def 
+        IMP_Minus_State_To_IMP_Minus_Minus_with_operands_a_b_def)
 
    hence "\<exists>prefix. length prefix \<le> length ((?sas_plus_plus_problem)\<^sub>\<V>\<^sub>+) + 1 
     \<and> is_serial_solution_for_problem (SAS_Plus_Plus_To_SAS_Plus ?sas_plus_plus_problem) 
@@ -116,7 +164,192 @@ proof -
       \<and> is_serial_solution_for_problem (IMP_Minus_to_SAS_Plus c I r G t) ?plan'"
      using plan_def prefix_def t'_def by(auto simp: IMP_Minus_to_SAS_Plus_def Let_def)
    thus ?thesis by (metis add.commute)
- qed
-    
+qed
+
+lemma not_in_superset_of_dom_then_None: "dom s \<subseteq> S \<Longrightarrow> x \<notin> S \<Longrightarrow> s x = None" by auto
+
+lemma all_bits_equal_then_equal: "x < 2 ^ n \<Longrightarrow> y < 2 ^ n \<Longrightarrow> (\<forall>i < n. nth_bit x i = nth_bit y i) 
+  \<Longrightarrow> x = y" sorry
+
+lemma SAS_Plus_to_IMP_Minus_correctness: 
+  assumes 
+    "dom I \<subseteq> set (IMP_Minus_Max_Constant.all_variables c)"
+    "dom G \<subseteq> set (IMP_Minus_Max_Constant.all_variables c)" 
+    "Max (ran G) < 2 ^ (t + max_input_bits c I r)" 
+    "is_serial_solution_for_problem (IMP_Minus_to_SAS_Plus c I r G t) plan"
+    "\<forall>s1. \<exists>s2. \<exists>t' \<le> t. (c, s1) \<Rightarrow>\<^bsup>t'\<^esup> s2" 
+  shows "\<exists>s1 s2 t'. t' \<le> t \<and> I \<subseteq>\<^sub>m Some \<circ> s1 \<and> G \<subseteq>\<^sub>m Some \<circ> s2 \<and> (c, s1)  \<Rightarrow>\<^bsup>t'\<^esup> s2" 
+proof -
+  let ?guess_range = "max_input_bits c I r"
+  let ?n = "t + ?guess_range + 1"
+  let ?c' = "IMP_Minus_To_IMP_Minus_Minus c ?n"
+  let ?I = "(IMP_Minus_initial_to_IMP_Minus_Minus I ?n ?guess_range) 
+    |` (set (enumerate_variables ?c'))"
+  let ?G = "(IMP_Minus_State_To_IMP_Minus_Minus_partial G ?n ?n) |` (set (enumerate_variables ?c'))"
+
+  have "finite (ran I)" "finite (ran G)" 
+    using \<open>dom I \<subseteq> set (IMP_Minus_Max_Constant.all_variables c)\<close> 
+      \<open>dom G \<subseteq> set (IMP_Minus_Max_Constant.all_variables c)\<close>
+    finite_set by(auto simp: finite_subset intro!: finite_ran)
+  
+  obtain plan' where "length plan' \<le> length plan
+    \<and> is_serial_solution_for_problem_sas_plus_plus (imp_minus_minus_to_sas_plus ?c' ?I ?G) plan'" 
+    using SAS_Plus_To_SAS_Plus_Plus 
+      \<open>is_serial_solution_for_problem (IMP_Minus_to_SAS_Plus c I r G t) plan\<close>
+    by (metis IMP_Minus_to_SAS_Plus_def imp_minus_minus_to_sas_plus_valid)
+
+  then obtain s1 s2 t' where "(?I|` set (enumerate_variables ?c')) \<subseteq>\<^sub>m s1"
+    "dom s1 = set (enumerate_variables ?c')"
+    "(?G|` set (enumerate_variables ?c')) \<subseteq>\<^sub>m s2" "t' \<le> length plan'" 
+    "(?c', s1) \<rightarrow>\<^bsup>t'\<^esup> (SKIP, s2)"
+    using sas_plus_plus_to_imp_minus_minus by fastforce
+
+  let ?s1' = "IMP_Minus_Minus_State_To_IMP_Minus s1 ?n" 
+  let ?s2' = "IMP_Minus_Minus_State_To_IMP_Minus s2 ?n"
+
+  have "s1 v = (IMP_Minus_State_To_IMP_Minus_Minus ?s1' ?n |` (set (enumerate_variables ?c'))) v" 
+    for v
+  proof(cases "v \<in> set (enumerate_variables ?c')")
+    case True
+    thus ?thesis
+    proof (cases "v \<in> dom ?I")
+      case True
+      hence "s1 v = ?I v" using \<open>(?I|` set (enumerate_variables ?c')) \<subseteq>\<^sub>m s1\<close> 
+        by(auto simp: map_le_def)
+      thus ?thesis using \<open>v \<in> set (enumerate_variables ?c')\<close> 
+          apply(auto simp: IMP_Minus_State_To_IMP_Minus_Minus_partial_def  
+              IMP_Minus_State_To_IMP_Minus_Minus_with_operands_a_b_def var_to_var_bit_eq_Some_iff
+              var_to_operand_bit_eq_Some_iff IMP_Minus_initial_to_IMP_Minus_Minus_def
+              IMP_Minus_State_To_IMP_Minus_Minus_partial_of_operand_bit_to_var
+              IMP_Minus_State_To_IMP_Minus_Minus_def
+              nth_bit_of_IMP_Minus_Minus_State_To_IMP_Minus 
+              split: option.splits)
+        using \<open>v \<in> dom ?I\<close> by(auto simp: map_comp_def IMP_Minus_initial_to_IMP_Minus_Minus_def 
+            IMP_Minus_State_To_IMP_Minus_Minus_partial_def
+            IMP_Minus_State_To_IMP_Minus_Minus_partial_of_operand_bit_to_var 
+            dest!: set_mp[OF IMP_Minus_To_IMP_Minus_Minus_variables] 
+            split: option.splits char.splits bool.splits)
+    next
+      case False
+      then obtain v' i where "v = var_bit_to_var (v', i) \<and> i < ?guess_range" using \<open>\<not>(v \<in> dom ?I)\<close>
+         \<open>v \<in> set (enumerate_variables ?c')\<close>
+        set_mp[OF IMP_Minus_To_IMP_Minus_Minus_variables \<open>v \<in> set (enumerate_variables ?c')\<close>]
+        apply(auto simp: IMP_Minus_initial_to_IMP_Minus_Minus_def map_comp_def
+            IMP_Minus_State_To_IMP_Minus_Minus_partial_def split: option.splits)
+        using leI by blast
+      thus ?thesis using \<open>v \<in> set (enumerate_variables ?c')\<close> 
+          \<open>dom s1 = set (enumerate_variables ?c')\<close>
+        by(auto simp: IMP_Minus_State_To_IMP_Minus_Minus_def 
+            nth_bit_of_IMP_Minus_Minus_State_To_IMP_Minus
+            IMP_Minus_State_To_IMP_Minus_Minus_with_operands_a_b_def split: option.splits)
+    qed
+  next
+    case False
+    thus ?thesis using \<open>dom s1 = set (enumerate_variables ?c')\<close> by auto
+  qed
+  hence "s1 = IMP_Minus_State_To_IMP_Minus_Minus ?s1' ?n |` (set (enumerate_variables ?c'))" by auto
+
+  have "I v = Some y \<Longrightarrow> ?s1' v = y" for v y 
+  proof -
+    assume "I v = Some y" 
+    hence "v \<in> set (IMP_Minus_Max_Constant.all_variables c)" 
+      using \<open>dom I \<subseteq> set (IMP_Minus_Max_Constant.all_variables c)\<close> by auto
+    hence "\<forall>i < ?n. var_bit_to_var (v, i) \<in> set (enumerate_variables ?c')" 
+      by(auto simp: var_bit_in_IMP_Minus_Minus_variables)
+    moreover hence "i < ?n \<longrightarrow> s1 (var_bit_to_var (v, i)) = ?I (var_bit_to_var (v, i))" for i
+      using \<open>(?I|` set (enumerate_variables ?c')) \<subseteq>\<^sub>m s1\<close> \<open>I v = Some y\<close>
+      by(auto simp: IMP_Minus_initial_to_IMP_Minus_Minus_def map_le_def
+          IMP_Minus_State_To_IMP_Minus_Minus_def dom_def
+          IMP_Minus_State_To_IMP_Minus_Minus_partial_def map_comp_def split: option.splits) 
+    ultimately show "?s1' v = y" using \<open>(?I|` set (enumerate_variables ?c')) \<subseteq>\<^sub>m s1\<close>
+       less_le_trans[OF initial_state_element_less_two_to_the_max_input_bits[where ?c=c and ?r=r]]
+       \<open>I v = Some y\<close> bit_at_index_geq_max_input_bits_is_zero_in_initial_state \<open>finite (ran I)\<close>
+      by(fastforce simp add: IMP_Minus_initial_to_IMP_Minus_Minus_def map_comp_def 
+          IMP_Minus_Minus_State_To_IMP_Minus_def power_add 
+          algebra_simps nth_append bit_list_to_nat_eq_nat_iff
+          IMP_Minus_State_To_IMP_Minus_Minus_partial_def split: if_splits option.splits)
+  qed
+  hence "I \<subseteq>\<^sub>m Some \<circ> ?s1'" by(auto simp: map_le_def)
+  
+  hence "t_small_step_fun t' 
+  (?c', IMP_Minus_State_To_IMP_Minus_Minus ?s1' ?n |` set (enumerate_variables ?c')) = (SKIP, s2)"
+    using \<open>(?c', s1) \<rightarrow>\<^bsup>t'\<^esup> (SKIP, s2)\<close> 
+      \<open>s1 = IMP_Minus_State_To_IMP_Minus_Minus ?s1' ?n |` (set (enumerate_variables ?c'))\<close>
+    by(auto simp: t_small_step_fun_t_small_step_equivalence)
+  moreover have "t_small_step_fun t' 
+    (?c', IMP_Minus_State_To_IMP_Minus_Minus ?s1' ?n |` set (enumerate_variables ?c')) 
+    = (fst (t_small_step_fun t' (?c', IMP_Minus_State_To_IMP_Minus_Minus ?s1' ?n)),
+       snd  (t_small_step_fun t' (?c', IMP_Minus_State_To_IMP_Minus_Minus ?s1' ?n)) 
+      |` set (enumerate_variables ?c'))" 
+    by (auto simp: t_small_step_fun_restrict_variables)
+  ultimately obtain s2' where "t_small_step_fun t' (?c', IMP_Minus_State_To_IMP_Minus_Minus ?s1' ?n)
+    = (SKIP, s2')" "s2' |` set (enumerate_variables ?c') = s2" by auto (metis prod.collapse)
+
+  moreover obtain t'' s2'' where "t'' \<le> t" "(c, ?s1') \<Rightarrow>\<^bsup>t''\<^esup> s2''" 
+    using \<open>\<forall>s1. \<exists>s2. \<exists>t' \<le> t. (c, s1) \<Rightarrow>\<^bsup>t'\<^esup> s2\<close> by blast
+  moreover have "?guess_range \<le> i \<Longrightarrow> s1 (var_bit_to_var (v, i)) \<noteq> Some One" for i v 
+  proof(cases "(var_bit_to_var (v, i)) \<in> set (enumerate_variables ?c')")
+    case True
+    assume "?guess_range \<le> i"
+    hence "?I (var_bit_to_var (v, i)) = Some Zero" 
+      using \<open>(var_bit_to_var (v, i)) \<in> set (enumerate_variables ?c')\<close>  
+      by(auto simp: IMP_Minus_initial_to_IMP_Minus_Minus_def 
+          IMP_Minus_State_To_IMP_Minus_Minus_partial_def 
+          dest!: set_mp[OF IMP_Minus_To_IMP_Minus_Minus_variables]
+          split: option.splits)
+    thus ?thesis using \<open>(?I|` set (enumerate_variables ?c')) \<subseteq>\<^sub>m s1\<close> by(auto simp: map_le_def dom_def)
+  next
+    case False
+    then show ?thesis using \<open>dom s1 = set (enumerate_variables ?c')\<close> by auto
+  qed
+   
+  moreover hence "finite (range (IMP_Minus_Minus_State_To_IMP_Minus s1 ?n))" 
+    "Max (range (IMP_Minus_Minus_State_To_IMP_Minus s1 ?n)) < 2 ^ ?guess_range" 
+    using all_bits_geq_k_Zero_then_IMP_Minus_Minus_State_To_IMP_Minus_range_limited by blast+
+  ultimately have "s2' = IMP_Minus_State_To_IMP_Minus_Minus s2'' ?n" 
+    using IMP_Minus_Minus_To_IMP_Minus_aux max_constant_less_two_to_the_max_input_bits
+    by(auto simp: power_add algebra_simps mult_2 trans_less_add2)
+
+  have "G v = Some y \<Longrightarrow> s2'' v = y" for v y 
+  proof -
+    assume "G v = Some y" 
+    hence "v \<in> set (IMP_Minus_Max_Constant.all_variables c)" 
+      using \<open>dom G \<subseteq> set (IMP_Minus_Max_Constant.all_variables c)\<close> by auto
+    hence "\<forall>i < ?n. var_bit_to_var (v, i) \<in> set (enumerate_variables ?c')" 
+      by(auto simp: var_bit_in_IMP_Minus_Minus_variables)
+    moreover hence "i < ?n \<longrightarrow> s2 (var_bit_to_var (v, i)) = ?G (var_bit_to_var (v, i))" for i
+      using \<open>(?G|` set (enumerate_variables ?c')) \<subseteq>\<^sub>m s2\<close> \<open>G v = Some y\<close>
+      by(auto simp: IMP_Minus_initial_to_IMP_Minus_Minus_def map_le_def
+          IMP_Minus_State_To_IMP_Minus_Minus_def dom_def
+          IMP_Minus_State_To_IMP_Minus_Minus_partial_def map_comp_def split: option.splits) 
+    moreover hence "i < ?n \<longrightarrow> s2' (var_bit_to_var (v, i)) = ?G (var_bit_to_var (v, i))" for i 
+      using \<open>s2' |` set (enumerate_variables ?c') = s2\<close> 
+        \<open>\<forall>i < ?n. var_bit_to_var (v, i) \<in> set (enumerate_variables ?c')\<close> by auto
+    ultimately have "i < ?n \<longrightarrow> map_option (\<lambda>x. nth_bit x i) (G v) = Some (nth_bit (s2'' v) i)" for i 
+      using  \<open>s2' = IMP_Minus_State_To_IMP_Minus_Minus s2'' ?n\<close> \<open>G v = Some y\<close>
+      by(auto simp: IMP_Minus_State_To_IMP_Minus_Minus_def 
+          IMP_Minus_State_To_IMP_Minus_Minus_partial_def
+          IMP_Minus_State_To_IMP_Minus_Minus_with_operands_a_b_def)
+    thus "s2'' v = y"
+      apply - apply(rule all_bits_equal_then_equal[where ?n = "?n"])
+      apply(insert IMP_Minus_space_growth[OF \<open>(c, ?s1') \<Rightarrow>\<^bsup>t''\<^esup> s2''\<close> 
+          \<open>finite (range (IMP_Minus_Minus_State_To_IMP_Minus s1 ?n))\<close>, where ?k="?guess_range"])
+      using \<open>Max (range (IMP_Minus_Minus_State_To_IMP_Minus s1 ?n)) < 2 ^ ?guess_range\<close>
+        max_constant_less_two_to_the_max_input_bits \<open>t'' \<le> t\<close>
+        apply simp
+        apply(rule less_le_trans[where ?y="2 ^ (t + max_input_bits c I r)"])
+         apply(auto simp: algebra_simps)
+        apply(rule less_le_trans[where ?y="2 ^ (t'' + max_input_bits c I r)"])
+      using \<open>G v = Some y\<close>  apply(auto)
+      apply(rule less_le_trans[where ?y="2 ^ (t + max_input_bits c I r)"])
+       apply (meson ran_def Max_ge \<open>finite (ran G)\<close> \<open>Max (ran G) < 2 ^ (t + max_input_bits c I r)\<close> 
+          le_less_trans ranI)
+      by simp
+  qed
+  hence "G \<subseteq>\<^sub>m Some \<circ> s2''" by(auto simp: map_le_def)
+
+  show ?thesis using \<open>t'' \<le> t\<close> \<open>(c, ?s1') \<Rightarrow>\<^bsup>t''\<^esup> s2''\<close> \<open>I \<subseteq>\<^sub>m Some \<circ> ?s1'\<close> \<open>G \<subseteq>\<^sub>m Some \<circ> s2''\<close>
+    by auto
+qed
 
 end
